revert some stuff

Clean/Tables/Fibonacci32Inductive.lean
@@ -11,9 +11,18 @@ def fib32 : ℕ → ℕ
   | 1 => 1
   | n + 2 => (fib32 n + fib32 (n + 1)) % 2^32
 
-def table : InductiveTable (F p) Addition32.Inputs unit where
+structure Row (F : Type) where
+  x: U32 F
+  y: U32 F
+
+instance : ProvableStruct Row where
+  components := [U32, U32]
+  to_components := fun { x, y } => .cons x (.cons y .nil)
+  from_components := fun (.cons x (.cons y .nil)) => { x, y }
+
+def table : InductiveTable (F p) Row unit where
   step row _ := do
-    let z ← subcircuit Gadgets.Addition32.circuit row
+    let z ← subcircuit Gadgets.Addition32.circuit { x := row.x, y := row.y }
     return { x := row.y, y := z }
 
   spec i row _ _ : Prop :=
@@ -28,10 +37,10 @@ def table : InductiveTable (F p) Addition32.Inputs unit where
     Addition32.circuit, Addition32.assumptions, Addition32.spec]
 
 -- the input is hard-coded to (0, 1)
-def formalTable (output : Addition32.Inputs (F p)) := table.toFormal { x := U32.from_byte 0, y := U32.from_byte 1 } output
+def formalTable (output : Row (F p)) := table.toFormal { x := U32.from_byte 0, y := U32.from_byte 1 } output
 
 -- The table's statement implies that the output row contains the nth Fibonacci number
-theorem tableStatement (output : Addition32.Inputs (F p)) : ∀ n > 0, ∀ trace,
+theorem tableStatement (output : Row (F p)) : ∀ n > 0, ∀ trace,
     (formalTable output).statement n trace → output.y.value = fib32 n := by
   intro n hn trace spec
   simp only [FormalTable.statement, formalTable, InductiveTable.toFormal, table] at spec
